More tidying, including removal of separate state type
Removing the state type (replacing it with just numbers) allows us to
dispense with the abstraction and representation functions for moving
backwards and forwards between states and numbers.

examples/computability/turingMachines/turing_machineScript.sml
@@ -64,10 +64,8 @@ val _ = Datatype `action = Wr0 | Wr1 | L | R`;
 
 val _ = Datatype `cell = Z | O `;
 
-val _ = Datatype `state = <| n : num |>`;
-
-val _ = Datatype `TM = <| state : state;
-                          prog : ((state # cell) |->  (state # action));
+val _ = Datatype `TM = <| state : num;
+                          prog : ((num # cell) |->  (num # action));
                           tape_l : cell list;
                           tape_h : cell;
                           tape_r : cell list
@@ -86,20 +84,14 @@ val INITIAL_TAPE_TM_def = Define `
 
 val INITIAL_TM_def = Define`
   INITIAL_TM p args =
-    INITIAL_TAPE_TM <| state := <|n:=0|>;  prog := p;tape_l := [];
+    INITIAL_TAPE_TM <| state := 0;  prog := p;tape_l := [];
                        tape_h := Z;tape_r := [] |>
                     (concatWith [Z] (MAP (GENLIST (K O)) args))`;
 
-val UPDATE_STATE_TIME = Define `UPDATE_STATE_TIME tm =
-  if (tm.state,tm.tape_h) IN FDOM tm.prog
-  then tm with <|state := (FST (tm.prog ' ((tm.state) ,(tm.tape_h)) )) |>
-  else (tm)
-                               `;
-
 val UPDATE_TAPE_def = Define `
   UPDATE_TAPE tm =
-    if (tm.state,tm.tape_h) IN FDOM tm.prog ∧ tm.state.n <> 0 then
-      let tm' = tm with state := FST (tm.prog ' ((tm.state) ,(tm.tape_h)) )
+    if (tm.state,tm.tape_h) IN FDOM tm.prog ∧ tm.state <> 0 then
+      let tm' = tm with state := FST (tm.prog ' (tm.state, tm.tape_h))
       in
         case SND (tm.prog ' (tm.state ,tm.tape_h)) of
           Wr0 => tm' with tape_h := Z
@@ -116,7 +108,7 @@ val UPDATE_TAPE_def = Define `
                  else tm' with <| tape_l := tm.tape_h::tm.tape_l;
                                   tape_h := HD tm.tape_r;
                                   tape_r := TL tm.tape_r |>
-    else tm with state := <|n:=0|>
+    else tm with state := 0
 `;
 
 val _ = overload_on("RUN",``FUNPOW UPDATE_TAPE``);
@@ -180,11 +172,7 @@ val DECODE_TM_TAPE_def = Define `
            (DECODE (nfst n), O , DECODE ( (nsnd n - 1) DIV 2))`;
 
 (* Halted definition and TM examples *)
-val HALTED_def = Define `HALTED tm <=> (tm.state.n = 0)`;
-
-val st_def= Define`st n : state = <| n := n  |>`;
-val _ = add_numeral_form(#"s", SOME "st");
-
+val HALTED_def = Define `HALTED tm <=> (tm.state = 0)`;
 
 (*
 
@@ -217,17 +205,13 @@ val NUM_TO_ACT_def = Define `
   (NUM_TO_ACT 2 = L) ∧
   (NUM_TO_ACT 3 = R) `;
 
-val STATE_TO_NUM_def = Define `STATE_TO_NUM a = a.n`;
-
-val NUM_TO_STATE_def = Define `NUM_TO_STATE n = <| n:=n |>`;
-
 val FULL_ENCODE_TM_def = Define `
-  FULL_ENCODE_TM tm = STATE_TO_NUM tm.state *, ENCODE_TM_TAPE tm
+  FULL_ENCODE_TM tm = tm.state *, ENCODE_TM_TAPE tm
 `;
 
 
 val FULL_DECODE_TM_def = Define `
-  FULL_DECODE_TM n = <| state:=  NUM_TO_STATE (nfst n);
+  FULL_DECODE_TM n = <| state:=  nfst n;
                         tape_l := FST (DECODE_TM_TAPE (nsnd n));
                         tape_h := FST (SND (DECODE_TM_TAPE (nsnd n)));
                         tape_r := SND (SND (DECODE_TM_TAPE (nsnd n)))|>
@@ -235,8 +219,8 @@ val FULL_DECODE_TM_def = Define `
 
 (* Perform action an move to state *)
 val UPDATE_ACT_S_TM_def = Define `UPDATE_ACT_S_TM s act tm =
-           let tm' = tm with
-                        <|  state := s |> in
+           let tm' = tm with state := s
+           in
                case act of
                    Wr0 => tm' with tape_h := Z
                  | Wr1 => tm' with tape_h := O
@@ -284,48 +268,52 @@ val ODD_MOD_TWO_lem = Q.store_thm ("ODD_MOD_TWO_lem",
   rpt strip_tac  >> fs[MOD_2] >> `~EVEN n` by metis_tac[EVEN_AND_ODD] >> rw[]);
 
 val containment_lem = Q.store_thm("containment_lem",
-`((OLEAST n. (NUM_TO_STATE (nfst n),CELL_NUM (nsnd n)) ∈ FDOM p) =
-  NONE) <=> (p = FEMPTY)`,
-rw[] >> eq_tac >> simp[] >> csimp[fmap_EXT] >>
-simp[EXTENSION,pairTheory.FORALL_PROD,NUM_TO_STATE_def] >> strip_tac >>
-qx_gen_tac `a` >> qx_gen_tac `b` >>
-`∃n. a= <| n := n|>  ` by metis_tac[theorem"state_literal_nchotomy"] >>
-`∃c. b = CELL_NUM c` by metis_tac[CELL_NUM_def,theorem"cell_nchotomy"] >> rw[] >>
-pop_assum (qspec_then `n *, c` mp_tac) >> simp[]);
+  `((OLEAST n. (nfst n,CELL_NUM (nsnd n)) ∈ FDOM p) = NONE) <=> (p = FEMPTY)`,
+  rw[] >> eq_tac >> simp[] >> csimp[fmap_EXT] >>
+  simp[EXTENSION,pairTheory.FORALL_PROD] >> strip_tac >>
+  qx_gen_tac `a` >> qx_gen_tac `b` >>
+  `∃c. b = CELL_NUM c` by metis_tac[CELL_NUM_def,theorem"cell_nchotomy"] >>
+  rw[] >>
+  pop_assum (qspec_then `a *, c` mp_tac) >> simp[]);
 
 
 val UPDATE_TAPE_ACT_STATE_TM_thm = Q.store_thm("UPDATE_TAPE_ACT_STATE_TM_thm",
-`∀ tm.(((tm.state) ,(tm.tape_h)) ∈ FDOM tm.prog)∧ (tm.state.n <> 0) ==> (UPDATE_ACT_S_TM (FST (tm.prog ' ((tm.state) ,(tm.tape_h)) ))
-  (SND (tm.prog ' ((tm.state) ,(tm.tape_h)) )) tm = UPDATE_TAPE tm)`,
-strip_tac >> fs[UPDATE_ACT_S_TM_def,UPDATE_TAPE_def]  );
+  `∀ tm.
+    ((tm.state , tm.tape_h) ∈ FDOM tm.prog) ∧ tm.state <> 0 ==>
+    (UPDATE_ACT_S_TM (FST (tm.prog ' (tm.state, tm.tape_h)))
+                     (SND (tm.prog ' (tm.state, tm.tape_h)))
+                     tm
+       =
+     UPDATE_TAPE tm)`,
+  strip_tac >> fs[UPDATE_ACT_S_TM_def,UPDATE_TAPE_def]  );
 
 val NUM_TO_ACT_TO_NUM = Q.store_thm("NUM_TO_ACT_TO_NUM[simp]",
-`((ACT_TO_NUM k) < 4) ==> (NUM_TO_ACT (ACT_TO_NUM k) = k)`,
-rw[NUM_TO_ACT_def,ACT_TO_NUM_def] >>
-`(ACT_TO_NUM k = 0) ∨ (ACT_TO_NUM k = 1) ∨(ACT_TO_NUM k = 2)∨(ACT_TO_NUM k = 3)` by simp[] >>rw[]>>
-EVAL_TAC >> Cases_on `k` >> rfs[ACT_TO_NUM_def] >> EVAL_TAC);
-
+  `((ACT_TO_NUM k) < 4) ==> (NUM_TO_ACT (ACT_TO_NUM k) = k)`,
+  rw[NUM_TO_ACT_def,ACT_TO_NUM_def] >>
+  `(ACT_TO_NUM k = 0) ∨ (ACT_TO_NUM k = 1) ∨(ACT_TO_NUM k = 2)∨
+   (ACT_TO_NUM k = 3)` by simp[] >>rw[]>>
+  EVAL_TAC >> Cases_on `k` >> rfs[ACT_TO_NUM_def] >> EVAL_TAC);
 val _ = export_rewrites ["NUM_CELL_def"]
+
 val TM_PROG_P_TAPE_H = Q.store_thm("TM_PROG_P_TAPE_H[simp]",
-`(tm with prog := p).tape_h = tm.tape_h`,
-fs[]);
+  `(tm with prog := p).tape_h = tm.tape_h`,
+  fs[]);
 
 val TM_PROG_P_STATE = Q.store_thm("TM_PROG_P_STATE[simp]",
-`(tm with prog := p).state = tm.state`,
-fs[]);
+  `(tm with prog := p).state = tm.state`,
+  fs[]);
 
 val UPDATE_TM_ARB_Q = Q.store_thm("UPDATE_TM_ARB_Q",
-`((tm.state,tm.tape_h) ∈ FDOM p)∧ (tm.state.n <> 0) ==> ((UPDATE_ACT_S_TM (FST (p ' (tm.state,tm.tape_h))) (SND (p ' (tm.state,tm.tape_h))) (tm with prog := q)) = ((UPDATE_TAPE (tm with prog := p)) with prog := q))`,
-rw[UPDATE_TAPE_def,UPDATE_ACT_S_TM_def] >>
-Cases_on `SND (p ' (tm.state,tm.tape_h))` >> simp[] )
+  `(tm.state,tm.tape_h) ∈ FDOM p ∧ tm.state <> 0 ==>
+   (UPDATE_ACT_S_TM (FST (p ' (tm.state,tm.tape_h)))
+                    (SND (p ' (tm.state,tm.tape_h)))
+                    (tm with prog := q) =
+    (UPDATE_TAPE (tm with prog := p)) with prog := q)`,
+  rw[UPDATE_TAPE_def,UPDATE_ACT_S_TM_def] >>
+  Cases_on `SND (p ' (tm.state,tm.tape_h))` >> simp[] )
 
-val NUM_TO_STATE_TO_NUM = Q.store_thm ("NUM_TO_STATE_TO_NUM[simp]",
-`NUM_TO_STATE (STATE_TO_NUM k) = k`,
-fs[STATE_TO_NUM_def,NUM_TO_STATE_def,theorem("state_component_equality")]  );
-
-val tm_with_prog = Q.store_thm("tm_with_prog",`tm with prog := tm.prog = tm`,simp[theorem("TM_component_equality")])
-
-
+val tm_with_prog = Q.store_thm("tm_with_prog",
+  `tm with prog := tm.prog = tm`,simp[theorem("TM_component_equality")])
 
 val FST_DECODE_TM_TAPE = Q.store_thm(
   "FST_DECODE_TM_TAPE[simp]",
@@ -337,10 +325,6 @@ val DECODE_EQ_NIL = Q.store_thm(
   `(DECODE n = []) ⇔ (n = 0)`,
   metis_tac[DECODE_EMPTY_lem, DECODE_def]);
 
-val STATE_TO_NUM_TO_STATE = Q.store_thm ("STATE_TO_NUM_TO_STATE[simp]",
-`STATE_TO_NUM (NUM_TO_STATE n) = n`,
-simp[STATE_TO_NUM_def,NUM_TO_STATE_def])
-
 val ODD_HD_DECODE = Q.store_thm(
   "ODD_HD_DECODE",
   `ODD n ==> (HD (DECODE n) = O)`,
@@ -350,7 +334,6 @@ val EVEN_HD_DECODE = Q.store_thm(
  "EVEN_HD_DECODE",
 `EVEN n ∧ (n ≠ 0)  ==> (HD (DECODE n) = Z)`,
 Cases_on `n` >> simp[DECODE_def] >> metis_tac[EVEN_AND_ODD,listTheory.HD]);
-
 
 val SND_SND_DECODE_TM_TAPE = Q.store_thm("SND_SND_DECODE_TM_TAPE",
 `SND (SND (DECODE_TM_TAPE (nsnd tmn))) = DECODE (nsnd (nsnd tmn) DIV 2)`,
@@ -384,19 +367,16 @@ val npair_lem = Q.store_thm("npair_lem",
   rpt strip_tac >> `∃j k. j *, k = n` by metis_tac[npair_cases] >> rw[] );
 
 val NUM_TO_CELL_TO_NUM = Q.store_thm("NUM_TO_CELL_TO_NUM",
-`((c=0) ∨ (c=1)) ==> (NUM_CELL (CELL_NUM c) = c)`,
-strip_tac >> rw[NUM_CELL_def,CELL_NUM_def]);
+  `((c=0) ∨ (c=1)) ==> (NUM_CELL (CELL_NUM c) = c)`,
+  strip_tac >> rw[NUM_CELL_def,CELL_NUM_def]);
 
-val FULL_ENCODE_TM_STATE = Q.store_thm("FULL_ENCODE_TM_STATE",
-`nfst (FULL_ENCODE_TM tm) = STATE_TO_NUM tm.state`,
-fs[FULL_ENCODE_TM_def]);
-
-
-
+val FULL_ENCODE_TM_STATE = Q.store_thm("FULL_ENCODE_TM_STATE[simp]",
+  `nfst (FULL_ENCODE_TM tm) = tm.state`,
+  fs[FULL_ENCODE_TM_def]);
 
 val tri_mono = Q.store_thm ("tri_mono[simp]",
-`∀x y. (tri x <= tri y) <=> (x <= y)`,
-Induct_on `y` >> simp[]  );
+  `∀x y. (tri x <= tri y) <=> (x <= y)`,
+  Induct_on `y` >> simp[]  );
 
 val npair_mono = Q.store_thm ("npair_mono[simp]",
   `(x *, y < x *, z )<=> (y<z)`,
@@ -409,24 +389,21 @@ val npair_mono = Q.store_thm ("npair_mono[simp]",
 
 
 val CELL_NUM_LEM1 = Q.store_thm("CELL_NUM_LEM1",
-`((∀n'. n' < n ⊗ c ⇒ (NUM_TO_STATE (nfst n'),CELL_NUM (nsnd n')) ∉ FDOM p )
-      ∧ ( (NUM_TO_STATE n,CELL_NUM c) ∈ FDOM p)) ==> ((c=0) ∨ (c=1))`,
-spose_not_then strip_assume_tac >> Cases_on `CELL_NUM c` >-
-               (`0<c` by simp[] >> metis_tac[nfst_npair,nsnd_npair,npair_mono,CELL_NUM_def]  ) >-
-               (`1<c` by simp[] >> metis_tac[nfst_npair,nsnd_npair,npair_mono,CELL_NUM_def]  ) );
-
-val TM_PROG_LEM_1 = Q.store_thm("TM_PROG_LEM_1",
-`((tm.prog \\ (a,b) = tm'.prog) ∧ (tm = tm') ) ==> ¬((a,b) ∈ FDOM tm.prog)`,
-strip_tac >> `tm.prog = tm'.prog` by simp[] >> rw[] >>
-`FDOM (tm.prog \\ (a,b)) = FDOM tm.prog DELETE (a,b)` by  simp[FDOM_DOMSUB] >>
-`(FDOM (tm.prog \\ (a,b)) = FDOM tm.prog)` by metis_tac[EQ_FDOM_SUBMAP] >>
-` FDOM tm.prog DELETE (a,b) = FDOM tm.prog` by  metis_tac[] >>  simp[DELETE_NON_ELEMENT] )
+  `(∀n'. n' < n ⊗ c ⇒ (nfst n',CELL_NUM (nsnd n')) ∉ FDOM p) ∧
+   (n,CELL_NUM c) ∈ FDOM p ==> (c=0) ∨ (c=1)`,
+  spose_not_then strip_assume_tac >> Cases_on `CELL_NUM c`
+  >- (`0<c` by simp[] >>
+      metis_tac[nfst_npair,nsnd_npair,npair_mono,CELL_NUM_def]) >>
+  `1<c` by simp[] >> metis_tac[nfst_npair,nsnd_npair,npair_mono,CELL_NUM_def]);
 
 val TM_ACT_LEM_1 = Q.store_thm("TM_ACT_LEM_1[simp]",
   `( (nsnd (nsnd (FULL_ENCODE_TM tm))) MOD 2) = NUM_CELL (tm.tape_h)`,
   simp[FULL_ENCODE_TM_def,ENCODE_TM_TAPE_def] >> rw[] >> Cases_on `tm.tape_h` >- fs[] >- EVAL_TAC)
 
-val _ = add_rule {term_name = "FULL_ENCODE_TM",fixity = Closefix, block_style = (AroundEachPhrase,(PP.CONSISTENT,0)),paren_style = OnlyIfNecessary,pp_elements = [TOK "⟦",TM,TOK"⟧"]}
+val _ = add_rule {term_name = "FULL_ENCODE_TM",fixity = Closefix,
+                  block_style = (AroundEachPhrase,(PP.CONSISTENT,0)),
+                  paren_style = OnlyIfNecessary,
+                  pp_elements = [TOK "⟦",TM,TOK"⟧"]}
 
 val FULL_ENCODE_IGNORES_PROGS = Q.store_thm("FULL_ENCODE_IGNORES_PROGS[simp]",
 `⟦tm with prog := p⟧ = ⟦tm⟧`,
@@ -436,47 +413,23 @@ val NUM_CELL_INJ = Q.store_thm("NUM_CELL_INJ",
 `(NUM_CELL a = NUM_CELL b) <=> (a = b)`,
 eq_tac >- (Cases_on ` a` >> Cases_on `b` >> rw[] ) >- (rw[]) )
 
-val lem_bar_foo = UPDATE_TM_ARB_Q |> Q.INST [`tm`|->`FULL_DECODE_TM ⟦tm⟧`,`q`|->`(FULL_DECODE_TM ⟦tm⟧).prog` ] |> SIMP_RULE(srw_ss())[]
-
-
-val NFST_ENCODE_TM = Q.store_thm("NFST_ENCODE_TM[simp]",
-`(nfst ⟦tm⟧) = STATE_TO_NUM tm.state`,
-simp[FULL_ENCODE_TM_def])
-
-val TM_PROG_P_P = Q.store_thm("TM_PROG_P_P[simp]",
-`(tm with prog := p).prog = p`,
-fs[]);
-
-
 val ACT_TO_NUM_LESS_4 = Q.store_thm("ACT_TO_NUM_LESS_4",
 `ACT_TO_NUM a < 4`,
 Cases_on `a` >> EVAL_TAC)
 
-
-val EVEN_PLUS_1_thm = Q.store_thm("EVEN_PLUS_1_thm",
-`ODD (2 * n + 1)`,
-`2*n + 1 = SUC (2*n)` by fs[] >> rw[ODD_DOUBLE ])
-
 val TWO_TIMES_DIV_TWO_thm = Q.store_thm("TWO_TIMES_DIV_TWO_thm[simp]",
-`2 *  n DIV 2 = n`,
-Induct_on `n` >> fs[] >>  `2* SUC n = 2*n+2` by fs[] >> rw[] >> `0 < 2` by fs[] >> `2*n + 2 = n*2 + 2` by fs[] >>
-`(n*2 +2) DIV 2 = n + 2 DIV 2` by fs[ADD_DIV_ADD_DIV]  >> `(2*n +2) DIV 2 = n + 2 DIV 2` by fs[] >> rw[] )
+  `2 *  n DIV 2 = n`,
+  metis_tac[DECIDE “0 < 2”, MULT_DIV, MULT_COMM]);
 
-val TWO_TIMES_P_ONE_DIV_TWO_thm = Q.store_thm("TWO_TIMES_P_ONE_DIV_TWO_thm[simp]",
-`(2 * n + 1) DIV 2 = n`,
-Induct_on `n` >> fs[] >> `2* SUC n = 2*n+2` by fs[] >> rw[] >> `0 < 2` by fs[] >> `2*n + 2 = n*2 + 2` by fs[] >> `(n*2 +3) DIV 2 = n + 3 DIV 2` by fs[ADD_DIV_ADD_DIV] >> `(2*n +3) DIV 2 = n + 3 DIV 2` by fs[] >> rw[])
+val TWO_TIMES_P_ONE_DIV_TWO_thm = Q.store_thm(
+  "TWO_TIMES_P_ONE_DIV_TWO_thm[simp]",
+  `(2 * n + 1) DIV 2 = n`,
+  metis_tac[DECIDE “1 < 2”, DIV_MULT, MULT_COMM]);
 
-
-val ENCODE_CONS_DECODE_ENCODE_thm = Q.store_thm("ENCODE_CONS_DECODE_ENCODE_thm[simp]",
-`ENCODE (h::DECODE (ENCODE t)) = ENCODE (h::t)`,
-fs[ENCODE_def,DECODE_def,ENCODE_DECODE_thm])
-
-val FST_SND_DECODE_TM_TAPE_FULL_EVEN = Q.store_thm("FST_SND_DECODE_TM_TAPE_FULL_EVEN",
-`EVEN (nsnd t) ==> (FST (SND (DECODE_TM_TAPE t)) = Z)`,rw[DECODE_TM_TAPE_def] )
-
-val FST_SND_DECODE_TM_TAPE_FULL_NEVEN = Q.store_thm("FST_SND_DECODE_TM_TAPE_FULL_NEVEN",
-`¬EVEN (nsnd t) ==> (FST (SND (DECODE_TM_TAPE t)) = O)`,rw[DECODE_TM_TAPE_def] )
-
+val ENCODE_CONS_DECODE_ENCODE_thm = Q.store_thm(
+  "ENCODE_CONS_DECODE_ENCODE_thm[simp]",
+  `ENCODE (h::DECODE (ENCODE t)) = ENCODE (h::t)`,
+  fs[ENCODE_def,DECODE_def,ENCODE_DECODE_thm]);
 
 val NFST_ENCODE_TM_TAPE = Q.store_thm("NFST_ENCODE_TM_TAPE[simp]",
 `nfst (ENCODE_TM_TAPE tm) = ENCODE tm.tape_l`,
@@ -484,10 +437,11 @@ rw[ENCODE_TM_TAPE_def]);
 
 val FST_SND_DECODE_TM_TAPE = Q.store_thm("FST_SND_DECODE_TM_TAPE[simp]",
 `FST (SND (DECODE_TM_TAPE (ENCODE_TM_TAPE tm))) = tm.tape_h`,
-rw[DECODE_TM_TAPE_def,ENCODE_TM_TAPE_def] >> fs[EVEN_MULT,EVEN_ADD] >> Cases_on `tm.tape_h` >> fs[])
+rw[DECODE_TM_TAPE_def,ENCODE_TM_TAPE_def] >> fs[EVEN_MULT,EVEN_ADD] >>
+Cases_on `tm.tape_h` >> fs[]);
 
 val NSND_ENCODE_TM_TAPE_DIV2 = Q.store_thm("NSND_ENCODE_TM_TAPE_DIV2[simp]",
 `(nsnd (ENCODE_TM_TAPE tm) DIV 2) = ENCODE tm.tape_r`,
-rw[ENCODE_TM_TAPE_def])
+rw[ENCODE_TM_TAPE_def]);
 
 val _ = export_theory();
